Steel.Repr: split fsti/fst

experiment/Experiment.Steel.Repr.ST.fst
@@ -1,299 +1,13 @@
 module Experiment.Steel.Repr.ST
 
-module U    = Learn.Util
-module M    = Experiment.Steel.Repr.M
-module L    = FStar.List.Pure
-module Uv   = FStar.Universe
-module Fl   = Learn.FList
-module Perm = Learn.Permutation
-
-open Experiment.Steel.Repr.M
-open Steel.Effect.Common
-
-
-type pre_t = Fl.ty_list
-type post_t (a : Type) = a -> Fl.ty_list
-
-type req_t (pre : pre_t) = Fl.flist pre -> prop
-type ens_t (pre : pre_t) (a : Type) (post : post_t a) = Fl.flist pre -> (x : a) -> Fl.flist (post x) -> prop
-
-let const_post (#a : Type) (ts : Fl.ty_list) : post_t a = fun _ -> ts
-let frame_post (#a : Type) (pt : post_t a) (fr : Fl.ty_list) : post_t a = fun (x : a) -> L.(pt x @ fr)
-
-noeq
-type prog_tree : (a : Type u#a) -> (pre : pre_t u#b) -> (post : post_t u#a u#b a) -> Type u#(1 + max a b) =
-  | Tequiv : (pre : Fl.ty_list) -> (post : Fl.ty_list) ->
-             (p : Perm.pequiv pre post) ->
-             prog_tree U.unit' pre (const_post post)
-  | Tframe : (a : Type u#a) -> (pre : Fl.ty_list) -> (post : post_t a) -> (frame : Fl.ty_list) ->
-             (f : prog_tree a pre post) ->
-             prog_tree a L.(pre @ frame) (frame_post post frame)
-  | Tspec  : (a : Type u#a) -> (pre : pre_t) -> (post : post_t a) ->
-             (req : req_t pre) -> (ens : ens_t pre a post) ->
-             prog_tree a pre post
-  | Tret   : (a : Type u#a) -> (x : a) -> (post : post_t a) ->
-             prog_tree a (post x) post
-  | Tbind  : (a : Type u#a) -> (b : Type u#a) ->
-             (pre : pre_t) -> (itm : post_t a) -> (post : post_t b) ->
-             (f : prog_tree a pre itm) -> (g : ((x : a) -> prog_tree b (itm x) post)) ->
-             prog_tree b pre post
-  | TbindP : (a : Type u#a) -> (b : Type u#a) ->
-             (pre : pre_t) -> (post : post_t b) ->
-             (wp : pure_wp a) -> (x : unit -> PURE a wp) -> (g : a -> prog_tree b pre post) ->
-             prog_tree b pre post
-
-
-(* TODO ? r can requires t == t0*) 
-unfold
-let match_prog_tree
-      (#a0 : Type u#a) (#pre0 : pre_t u#b) (#post0 : post_t u#a u#b a0)
-      (t0 : prog_tree a0 pre0 post0)
-      (r : (a : Type u#a) -> (pre : pre_t u#b) -> (post : post_t u#a u#b a) ->
-           (t : prog_tree a pre post) -> Type u#c)
-      (c_Tequiv : (pre : Fl.ty_list) -> (post : Fl.ty_list) ->
-                  (p : Perm.pequiv pre post) ->
-                  Pure (r _ _ _ (Tequiv pre post p))
-                       (requires a0 == U.unit' /\ pre0 == pre /\ post0 == const_post post /\
-                                 t0 == Tequiv pre post p)
-                       (ensures fun _ -> True))
-      (c_Tframe : (a : Type) -> (pre : pre_t) -> (post : post_t a) -> (frame : Fl.ty_list) ->
-                  (f : prog_tree a pre post {f << t0}) ->
-                  Pure (r _ _ _ (Tframe a pre post frame f))
-                       (requires a0 == a /\ pre0 == L.(pre @ frame) /\
-                                 post0 == frame_post post frame /\
-                                 t0 == Tframe a pre post frame f)
-                       (ensures fun _ -> True))
-      (c_Tspec  : (a : Type) -> (pre : pre_t) -> (post : post_t a) ->
-                  (req : req_t pre) -> (ens : ens_t pre a post) ->
-                  Pure (r _ _ _ (Tspec a pre post req ens))
-                       (requires a0 == a /\ pre0 == pre /\
-                                 post0 == post /\
-                                 t0 == Tspec a pre post req ens)
-                       (ensures fun _ -> True))
-      (c_Tret   : (a : Type) -> (x : a) -> (post : post_t a) ->
-                  Pure (r _ _ _ (Tret a x post))
-                       (requires a0 == a /\ pre0 == post x /\ post0 == post /\
-                                 t0 == Tret a x post)
-                       (ensures fun _ -> True))
-      (c_Tbind  : (a : Type) -> (b : Type) ->
-                  (pre : pre_t) -> (itm : post_t a) -> (post : post_t b) ->
-                  (f : prog_tree a pre itm {f << t0}) ->
-                  (g : ((x : a) -> prog_tree b (itm x) post) {forall (x : a) . {:pattern (g x)} g x << t0}) ->
-                  Pure (r _ _ _ (Tbind a b pre itm post f g))
-                       (requires a0 == b /\ pre0 == pre /\ post0 == post /\
-                                 t0 == Tbind a b pre itm post f g)
-                       (ensures fun _ -> True))
-      (c_TbindP : (a : Type) -> (b : Type) ->
-                  (pre : pre_t) -> (post : post_t b) ->
-                  (wp : pure_wp a) -> (x : (unit -> PURE a wp)) ->
-                  (g : (a -> prog_tree b pre post) {forall (x : a) . {:pattern (g x)} g x << t0}) ->
-                  Pure (r _ _ _ (TbindP a b pre post wp x g))
-                       (requires a0 == b /\ pre0 == pre /\ post0 == post /\
-                                 t0 == TbindP a b pre post wp x g)
-                       (ensures fun _ -> True))
-  : r _ _ _ t0
-  = match t0 as t returns r _ _ _ t with
-    | Tequiv pre post p           -> c_Tequiv pre post p
-    | Tframe a pre post frame f   -> c_Tframe a pre post frame f
-    | Tspec  a pre post req ens   -> c_Tspec  a pre post req ens
-    | Tret   a x post             -> c_Tret   a x post
-    | Tbind  a b pre itm post f g -> c_Tbind  a b pre itm post f g
-    | TbindP a b pre post wp x g  -> c_TbindP a b pre post wp x g
-
-
-let bind (#a : Type) (#b : Type) (#pre : pre_t) (#itm : post_t a) (#post : post_t b)
-         (f : prog_tree a pre itm) (g : (x:a) -> prog_tree b (itm x) post)
-  : prog_tree b pre post
-  = Tbind a b pre itm post f g
-
-(* TODO? generalize Experiment.Steel.Repr.M.bind_req... *)
-let rec tree_req (#a : Type) (#pre : pre_t) (#post : post_t a) (t : prog_tree a pre post)
-  : Tot (req_t pre) (decreases t)
-  = match t with
-  | Tequiv _ _ _ ->
-             (fun sl0 -> True)
-  | Tframe _ pre _ frame f ->
-             (fun sl0 -> tree_req f (Fl.splitAt_ty pre frame sl0)._1)
-  | Tspec _  _ _  req _ ->
-             req
-  | Tret _ _ _ ->
-             (fun sl0 -> True)
-  | Tbind a _  _ itm _  f g ->
-             (fun sl0 -> tree_req f sl0 /\
-               (forall (x : a) (sl1 : Fl.flist (itm x)) . tree_ens f sl0 x sl1 ==> tree_req (g x) sl1))
-  | TbindP a _  _ _  wp _ g ->
-             (fun sl0 -> wp (fun (x : a) -> tree_req (g x) sl0) /\ True)
-
-and tree_ens (#a : Type) (#pre : pre_t) (#post : post_t a) (t : prog_tree a pre post)
-  : Tot (ens_t pre a post) (decreases t)
-  = match t with
-  | Tequiv _ post p ->
-             (fun sl0 _ sl1 ->
-               sl1 == Fl.apply_pequiv p sl0)
-  | Tframe a  pre post frame f ->
-             (fun sl0 x sl1 ->
-               let sl0', frame0 = Fl.splitAt_ty pre      frame sl0 in
-               let sl1', frame1 = Fl.splitAt_ty (post x) frame sl1 in
-               frame1 == frame0 /\ tree_ens f sl0' x sl1')
-  | Tspec _  _ _  _ ens ->
-             ens
-  | Tret _ x post ->
-             (fun sl0 x' sl1 -> x' == x /\ sl1 == sl0)
-  | Tbind a _  _ itm _  f g ->
-             (fun sl0 y sl2 ->
-               (exists (x : a) (sl1 : Fl.flist (itm x)) . tree_ens f sl0 x sl1 /\ tree_ens (g x) sl1 y sl2))
-  | TbindP a _  _ _  wp _ g ->
-             (fun sl0 y sl1 -> (exists (x : a) . as_ensures wp x /\ tree_ens (g x) sl0 y sl1))
-
-
-(***** Shape *)
-
-noeq
-type shape_tree : (pre_n : nat) -> (post_n : nat) -> Type =
-  | Sequiv : (n : nat) -> (p : Perm.perm_f n) ->
-             shape_tree n n
-  | Sframe : (pre_n : nat) -> (post_n : nat) -> (frame_n : nat) ->
-             (f : shape_tree pre_n post_n) ->
-             shape_tree (pre_n + frame_n) (post_n + frame_n)
-  | Sspec  : (pre_n : nat) -> (post_n : nat) ->
-             shape_tree pre_n post_n
-  | Sret   : (n : nat) ->
-             shape_tree n n
-  | Sbind  : (pre_n : nat) -> (itm_n : nat) -> (post_n : nat) ->
-             (f : shape_tree pre_n itm_n) -> (g : shape_tree itm_n post_n) ->
-             shape_tree pre_n post_n
-  | SbindP : (pre_n : nat) -> (post_n : nat) ->
-             (g : shape_tree pre_n post_n) ->
-             shape_tree pre_n post_n
-
-let post_has_len (#a : Type) (post : post_t a) (len : nat) : prop = forall (x : a) . L.length (post x) = len
-
-let rec prog_has_shape (#a : Type u#a) (#pre : pre_t u#b) (#post : post_t u#a u#b a)
-                       (t : prog_tree a pre post)
-                       (#post_n : nat) (s : shape_tree (L.length pre) post_n)
-  : Pure prop (requires True)
-              (ensures fun p -> p ==> post_has_len post post_n)
-              (decreases t)
-  =
-    post_has_len post post_n /\
-    (match t returns prop with
-    | Tequiv pre post p           -> post_n = L.length pre /\ s == Sequiv _ p
-    | Tframe _ pre post frame f   -> exists (post'_n : nat)
-                                      (s_f : shape_tree (L.length pre) post'_n) .
-                                    post_n = post'_n + L.length frame /\
-                                    s == Sframe (L.length pre) post'_n (L.length frame) s_f /\
-                                    prog_has_shape f s_f
-    | Tspec  _ pre post _ _       -> s == Sspec  (L.length pre) post_n /\
-                                    (forall (x : a) . L.length (post x) == post_n)
-    | Tret   _ _ post             -> post_n = L.length pre /\
-                                    s == Sret   _
-    | Tbind  a b pre itm post f g -> exists (itm_n : nat)
-                                      (s_f : shape_tree (L.length pre) itm_n)
-                                      (s_g : shape_tree itm_n          post_n) .
-                                    s == Sbind _ _ _ s_f s_g /\
-                                    prog_has_shape f s_f /\
-                                    (forall (x : a) . prog_has_shape (g x) s_g)
-    | TbindP a _ pre post _ _ g   -> exists (s_g : shape_tree (L.length pre) post_n) .
-                                    s == SbindP _ _ s_g /\
-                                   (forall (x : a) . prog_has_shape (g x) s_g)
-    )
-
-let rec prog_has_shape' (#a : Type u#a) (#pre : pre_t u#b) (#post : post_t u#a u#b a)
-                        (t : prog_tree a pre post)
-                        (#post_n : nat) (s : shape_tree (L.length pre) post_n)
-  : Pure prop (requires True) (ensures fun p -> p <==> prog_has_shape t s) (decreases t)
-  = match t returns prop with
-  | Tequiv pre post p           -> (match s with
-                                  | Sequiv _ p' -> p' == p
-                                  | _ -> False)
-  | Tframe _ pre post frame f   -> (match s with
-                                  | Sframe pre_n post_n frame_n s_f ->
-                                      pre_n   = L.length pre /\
-                                      frame_n = L.length frame /\
-                                      prog_has_shape' f s_f
-                                  | _ -> False)
-  | Tspec  _ pre post  _ _      -> (match s with
-                                  | Sspec  pre_n post_n ->
-                                     (forall (x : a) . post_n = L.length (post x))
-                                  | _ -> False)
-  | Tret   _ _ post             -> (match s with
-                                  | Sret   _ -> (forall (x : a) . post_n = L.length (post x))
-                                  | _ -> False)
-  | Tbind  a b pre itm post f g -> (match s with
-                                  | Sbind _ itm_n _ s_f s_g ->
-                                      prog_has_shape' f s_f /\
-                                      (forall (x : a) . prog_has_shape' (g x) s_g) /\
-                                      (forall (y : b) . post_n = L.length (post y))
-                                  | _ -> False)
-  | TbindP a b pre post _ _ g   -> (match s with
-                                  | SbindP _ _ s_g ->
-                                      (forall (x : a) . prog_has_shape' (g x) s_g) /\
-                                      (forall (y : b) . post_n = L.length (post y))
-                                  | _ -> False)
-
-
-noeq
-type prog_shape (#a : Type) (#pre : pre_t) (#post : post_t a) (t : prog_tree a pre post) = {
-  post_len : (l : nat {post_has_len post l});
-  shp      : (s : shape_tree (L.length pre) post_len {prog_has_shape t s});
-}
-
-unfold
-let mk_prog_shape (#a : Type) (#pre : pre_t) (#post : post_t a) (t : prog_tree a pre post)
-                  (#post_len : nat) (shp : shape_tree (L.length pre) post_len {prog_has_shape t shp})
-  : prog_shape t =
-  { post_len; shp}
-
-
-(*** Repr.M --> Repr.ST *)
-
+module L = FStar.List.Pure
 module T = FStar.Tactics
 open FStar.Calc
 
-let post_ST_of_M (#a : Type) (post : M.post_t a) : post_t a
-  = fun (x : a) -> vprop_list_sels_t (post x)
 
-let rec repr_ST_of_M (#a : Type u#a) (t : M.prog_tree a)
-                     (#pre0 : M.pre_t) (#post0 : M.post_t a) (c : M.tree_cond t pre0 post0)
-  : Tot (prog_tree a (vprop_list_sels_t pre0) (post_ST_of_M post0))
-        (decreases t)
-  = match c with
-  | TCspec #a #pre #post #req #ens  pre' post' frame  p0 p1 ->
-             Tequiv (vprop_list_sels_t pre') (vprop_list_sels_t L.(pre@frame)) (vequiv_sl p0);;
-             (**) L.map_append Mkvprop'?.t pre frame;
-             x <-- Tframe a (vprop_list_sels_t pre) (post_ST_of_M post) (vprop_list_sels_t frame)
-                 (Tspec a (vprop_list_sels_t pre) (post_ST_of_M post) req ens);
-             (**) L.map_append Mkvprop'?.t (post x) frame;
-             Tequiv (vprop_list_sels_t L.(post x @ frame))
-                    (vprop_list_sels_t (post' x))
-                    (vequiv_sl (p1 x));;
-             Tret _ x (post_ST_of_M post')
-  | TCret #a #x  pre post  p ->
-             Tequiv (vprop_list_sels_t pre) (vprop_list_sels_t (post x)) (vequiv_sl p);;
-             Tret _ x (post_ST_of_M post)
-  | TCbind #a #b #f #g  pre itm post  cf cg ->
-             x <-- repr_ST_of_M f cf;
-             repr_ST_of_M (g x) (cg x)
-  | TCbindP #a #b #wp #x #g  pre post  cg ->
-             TbindP a b _ _ wp x (fun x -> repr_ST_of_M (g x) (cg x))
+(**** soundness of M --> ST *)
 
-
-let rec shape_ST_of_M (#pre_n : nat) (#post_n : nat) (s : M.shape_tree pre_n post_n)
-  : Tot (shape_tree pre_n post_n) (decreases s)
-  = match s with
-  | M.Sspec pre_n post_n frame_n p0 p1 ->
-        Sbind _ _ _ (Sequiv (pre_n  + frame_n) p0) (
-        Sbind _ _ _ (Sframe pre_n post_n frame_n (Sspec  pre_n post_n)) (
-        Sbind _ _ _ (Sequiv (post_n + frame_n) p1)
-                    (Sret   (post_n + frame_n))))
-  | M.Sret n p ->
-        Sbind _ _ _ (Sequiv n p) (Sret n)
-  | M.Sbind _ _ _ f g -> Sbind  _ _ _ (shape_ST_of_M f) (shape_ST_of_M g)
-  | M.SbindP _ _ g    -> SbindP _ _ (shape_ST_of_M g)
-                    
-
-
-(***** soundness of M --> ST *)
+(***** Spec *)
 
 let norm_tree_spec () : T.Tac unit
   = T.norm [delta_only [`%repr_ST_of_M; `%post_ST_of_M; `%bind; `%tree_req; `%tree_ens; `%const_post];
@@ -301,7 +15,7 @@ let norm_tree_spec () : T.Tac unit
             delta_qualifier ["unfold"];
             zeta; iota; simplify]
 
-#push-options "--z3rlimit 15"
+#push-options "--z3rlimit 15 --ifuel 1"
 let repr_ST_of_M__TCspec_ens
       #a #pre #post (req : M.req_t pre) (ens : M.ens_t pre a post)
       (pre' : M.pre_t) (post' : M.post_t a) (frame : vprop_list)
@@ -345,11 +59,12 @@ let repr_ST_of_M__TCspec_ens
 #pop-options
 
 
-#push-options "--z3rlimit 30"
+#push-options "--z3rlimit 30 --ifuel 1"
 let rec repr_ST_of_M_req (#a : Type) (t : M.prog_tree a)
                          (#pre : M.pre_t) (#post : M.post_t a) (c : M.tree_cond t pre post)
                          (sl0 : sl_t pre)
   : Lemma (ensures M.tree_req t c sl0 <==> tree_req (repr_ST_of_M t c) sl0)
+          (decreases t)
   = match c as c returns squash (M.tree_req t c sl0 <==> tree_req (repr_ST_of_M t c) sl0) with
   | TCspec #a #pre #post #req #ens  pre' post' frame  p0 p1 ->
              L.map_append Mkvprop'?.t pre frame;
@@ -431,6 +146,7 @@ and repr_ST_of_M_ens (#a : Type) (t : M.prog_tree a)
                      (#pre : M.pre_t) (#post : M.post_t a) (c : M.tree_cond t pre post)
                      (sl0 : sl_t pre) (res : a) (sl1 : sl_t (post res))
   : Lemma (ensures M.tree_ens t c sl0 res sl1 <==> tree_ens (repr_ST_of_M t c) sl0 res sl1)
+          (decreases t)
   = match c as c returns squash (M.tree_ens t c sl0 res sl1 <==> tree_ens (repr_ST_of_M t c) sl0 res sl1) with
     | TCspec #a #pre #post #req #ens  pre' post' frame  p0 p1 ->
              L.map_append Mkvprop'?.t pre frame;
@@ -517,6 +233,8 @@ and repr_ST_of_M_ens (#a : Type) (t : M.prog_tree a)
             }
 #pop-options
 
+
+(***** Shape *)
 
 let repr_ST_of_M_shape__norm : list norm_step =
   [delta_only [`%prog_has_shape'; `%repr_ST_of_M; `%shape_ST_of_M; `%bind];
