experiment/Experiment.Steel.Repr.M.fsti
@@ -1,0 +1,434 @@
+module Experiment.Steel.Repr.M
+
+module U    = Learn.Util
+module L    = FStar.List.Pure
+module Dl   = Learn.DList
+module Fl   = Learn.FList
+module Ll   = Learn.List
+module Mem  = Steel.Memory
+module Perm = Learn.Permutation
+module FExt = FStar.FunctionalExtensionality
+
+open FStar.Calc
+open FStar.Classical.Sugar
+
+open Steel.Effect
+open Steel.Effect.Atomic
+
+irreducible let __tree_reduce__ : unit = ()
+
+
+(***** [vprop_list] *)
+
+type vprop_list = list vprop'
+
+let rec vprop_of_list (vpl : vprop_list) : vprop =
+  match vpl with
+  | [] -> emp
+  | v :: vs -> VStar (VUnit v) (vprop_of_list vs)
+
+val vprop_of_list_can_be_split (vs : vprop_list) (i : nat {i < L.length vs})
+  : Lemma (can_be_split (vprop_of_list vs) (VUnit (L.index vs i)))
+
+let rec flatten_vprop_aux (vp : vprop) (acc : vprop_list) : GTot vprop_list =
+  match vp with
+  | VUnit vp' -> vp' :: acc
+  | VStar vp0 vp1 -> flatten_vprop_aux vp0 (flatten_vprop_aux vp1 acc)
+
+let flatten_vprop (vp : vprop) : GTot vprop_list = flatten_vprop_aux vp []
+
+val flatten_vprop_aux_eq (vp : vprop) (acc : vprop_list)
+  : Lemma (flatten_vprop_aux vp acc == L.(flatten_vprop vp @ acc))
+
+val flatten_vprop_VStar (vp0 vp1 : vprop)
+  : Lemma (flatten_vprop (VStar vp0 vp1) == L.(flatten_vprop vp0 @ flatten_vprop vp1))
+
+val vprop_of_list_append (vs0 vs1 : vprop_list)
+  : Lemma (equiv (vprop_of_list L.(vs0@vs1)) (vprop_of_list vs0 `star` vprop_of_list vs1))
+
+val vprop_equiv_flat (vp : vprop)
+  : Lemma (equiv (vprop_of_list (flatten_vprop vp)) vp)
+
+
+(* ALT? dependent arrrow Fin.fin n -> _ *)
+
+[@@ __tree_reduce__]
+let vprop_list_sels_t : vprop_list -> Dl.ty_list =
+  L.map Mkvprop'?.t
+
+unfold
+let sl_t (vs : vprop_list) : Type = Fl.flist (vprop_list_sels_t vs)
+
+unfold
+let sl_list (vs : vprop_list) : Type = Dl.dlist (vprop_list_sels_t vs)
+
+let vprop_list_sels_t_eq (vs : vprop_list) (i : nat {i < L.length vs})
+  : Lemma (ensures L.index (vprop_list_sels_t vs) i == (L.index vs i).t)
+          [SMTPat (L.index (vprop_list_sels_t vs) i)]
+  = Ll.map_index Mkvprop'?.t vs i
+
+let rec vpl_sels (vs : vprop_list) (sl : t_of (vprop_of_list vs))
+  : Tot (sl_list vs) (decreases vs)
+  = match (|vs, sl|) <: (vs : vprop_list & t_of (vprop_of_list vs))  with
+  | (|[], _|) -> Dl.DNil
+  | (|v0 :: vs, (x0, xs)|) -> Dl.DCons v0.t x0 _ (vpl_sels vs xs)
+
+unfold
+let vpl_sels_f (vs : vprop_list) (sl : t_of (vprop_of_list vs)) : sl_t vs
+  = Fl.flist_of_d (vpl_sels vs sl)
+
+unfold
+let rmem_sl_list (#p:vprop) (vs : vprop_list)
+    (h:rmem p{FStar.Tactics.with_tactic selector_tactic (can_be_split p (vprop_of_list vs) /\ True)})
+  : GTot (sl_list vs)
+  = vpl_sels vs (h (vprop_of_list vs))
+
+unfold let rmem_sels (#p:vprop) (vs : vprop_list)
+    (h:rmem p{FStar.Tactics.with_tactic selector_tactic (can_be_split p (vprop_of_list vs) /\ True)})
+  : GTot (sl_t vs)
+  = Fl.flist_of_d (rmem_sl_list vs h)
+
+
+unfold
+let split_vars (vs0 vs1 : vprop_list) (xs : sl_t (vs0 @ vs1))
+  : sl_t vs0 & sl_t vs1
+  =
+    (**) Ll.map_append Mkvprop'?.t vs0 vs1;
+    Fl.splitAt_ty (vprop_list_sels_t vs0) (vprop_list_sels_t vs1) xs
+
+unfold
+let split_vars_list (vs0 vs1 : vprop_list) (xs : sl_list (vs0 @ vs1))
+  : sl_list vs0 & sl_list vs1
+  =
+    (**) Ll.map_append Mkvprop'?.t vs0 vs1;
+    Dl.splitAt_ty (vprop_list_sels_t vs0) (vprop_list_sels_t vs1) xs
+
+let split_vars__cons (v0 : vprop') (vs0 vs1 : vprop_list) (x0 : v0.t) (xs : sl_list L.(vs0@vs1))
+  : Lemma (ensures split_vars_list (v0 :: vs0) vs1 (Dl.DCons v0.t x0 (vprop_list_sels_t L.(vs0@vs1)) xs)
+               == (let xs0, xs1 = split_vars_list vs0 vs1 xs in
+                   Dl.DCons v0.t x0 (vprop_list_sels_t vs0) xs0, xs1))
+  = Ll.map_append Mkvprop'?.t vs0 vs1
+
+
+(***** [vequiv] *)
+
+let vequiv : vprop_list -> vprop_list -> Type = Perm.pequiv #vprop'
+
+unfold
+let vequiv_sl (#vs0 #vs1 : vprop_list) (f : vequiv vs0 vs1)
+  : Perm.pequiv (vprop_list_sels_t vs0) (vprop_list_sels_t vs1)
+  = Perm.map_apply_r f Mkvprop'?.t vs0;
+    U.cast #(Perm.perm_f (L.length vs0)) (Perm.perm_f (L.length (vprop_list_sels_t vs0))) f    
+
+unfold
+let extract_vars (#src #dst : vprop_list)
+                 (p : vequiv src dst)
+                 (xs : sl_t src)
+  : sl_t dst
+  =
+    Fl.apply_pequiv (vequiv_sl p) xs
+
+unfold
+let extract_vars_f (src dst frame : vprop_list)
+                   (p : vequiv src L.(dst@frame))
+                   (xs : sl_t src)
+  : sl_t dst & sl_t frame
+  =
+    split_vars dst frame (extract_vars p xs)
+
+let extract_vars_sym_l (#vs0 #vs1 : vprop_list) (f : vequiv vs0 vs1) (xs : sl_t vs0)
+  : Lemma (extract_vars (Perm.pequiv_sym f) (extract_vars f xs) == xs)
+  =
+    Fl.apply_pequiv_sym_l (vequiv_sl f) xs
+
+/// applying a permutation on the context's vprop
+
+val steel_change_vequiv (#vs0 #vs1 : vprop_list) (#opened:Mem.inames) (f : vequiv vs0 vs1)
+  : SteelGhost unit opened (vprop_of_list vs0) (fun () -> vprop_of_list vs1)
+      (requires fun _ -> True)
+      (ensures fun h0 () h1 -> rmem_sels vs1 h1 == extract_vars f (rmem_sels vs0 h0))
+
+(*** [prog_tree] *)
+
+type pre_t = vprop_list
+type post_t (a : Type) = a -> vprop_list
+
+type req_t (pre : pre_t) = sl_t pre -> prop
+type ens_t (pre : pre_t) (a : Type) (post : post_t a) = sl_t pre -> (x : a) -> sl_t (post x) -> prop
+
+type repr_steel_t (a : Type)
+       (pre : pre_t) (post : post_t a)
+       (req : req_t pre) (ens : ens_t pre a post) : Type
+  = unit -> Steel a
+             (vprop_of_list pre) (fun x -> vprop_of_list (post x))
+             (requires fun h0      -> req (rmem_sels pre h0))
+             (ensures  fun h0 x h1 -> ens (rmem_sels pre h0) x (rmem_sels (post x) h1))
+
+noeq
+type prog_tree : (a : Type u#a) -> Type u#(max (a+1) 2) =
+  | Tspec  : (a : Type u#a) -> (pre : pre_t) -> (post : post_t a) ->
+             (req : req_t pre) -> (ens : ens_t pre a post) ->
+             prog_tree a
+  | Tret   : (a : Type u#a) -> (x : a) -> prog_tree a
+  | Tbind  : (a : Type u#a) -> (b : Type u#a) ->
+             (f : prog_tree a) -> (g : a -> prog_tree b) ->
+             prog_tree b
+  | TbindP : (a : Type u#a) -> (b : Type u#a) ->
+             (wp : pure_wp a) -> (x : unit -> PURE a wp) -> (g : a -> prog_tree b) ->
+             prog_tree b
+
+
+(**** slprop unification conditions *)
+
+(* TODO:
+   - ? equalities vs vequiv
+      + Tspec : post x == post' x @ frame, allow shuffle at the end
+   - ~pr ! allow assumptions -> VC
+   - ALT: recursively defined type *)
+
+noeq
+type tree_cond : (#a : Type u#a) -> (t : prog_tree a) -> (pre : pre_t) -> (post : post_t a) -> Type u#(max (a+1) 2) =
+  | TCspec  : (#a : Type u#a) -> (#pre : pre_t) -> (#post : post_t a) -> (#req : req_t pre) -> (#ens : ens_t pre a post) ->
+              (pre' : pre_t) -> (post' : post_t a) -> (frame : vprop_list) ->
+              (p0 : vequiv pre' L.(pre @ frame)) ->
+              (p1 : ((x : a) -> vequiv (post x @ frame) (post' x))) ->
+              tree_cond (Tspec a pre post req ens) pre' post'
+  | TCret   : (#a : Type u#a) -> (#x : a) ->
+              (pre : pre_t) -> (post : post_t a) ->
+              (p : vequiv pre (post x)) ->
+              tree_cond (Tret a x) pre post
+  | TCbind  : (#a : Type u#a) -> (#b : Type u#a) -> (#f : prog_tree a) -> (#g : (a -> prog_tree b)) ->
+              (pre : pre_t) -> (itm : post_t a) -> (post : post_t b) ->
+              (cf : tree_cond f pre itm) -> (cg : ((x : a) -> tree_cond (g x) (itm x) post)) ->
+              tree_cond (Tbind a b f g) pre post
+  | TCbindP : (#a : Type u#a) -> (#b : Type u#a) ->
+              (#wp : pure_wp a) -> (#x : (unit -> PURE a wp)) -> (#g : (a -> prog_tree b)) ->
+              (pre : pre_t) -> (post : post_t b) ->
+              (cg : ((x : a) -> tree_cond (g x) pre post)) ->
+              tree_cond (TbindP a b wp x g) pre post
+
+(**** Shape *)
+
+noeq
+type shape_tree : (pre_n : nat) -> (post_n : nat) -> Type =
+  | Sspec  : (pre_n : nat) -> (post_n : nat) -> (frame_n : nat) ->
+             (p0 : Perm.perm_f (pre_n  + frame_n)) ->
+             (p1 : Perm.perm_f (post_n + frame_n)) ->
+             shape_tree (pre_n + frame_n) (post_n + frame_n)
+  | Sret   : (n : nat) -> (p : Perm.perm_f n) ->
+             shape_tree n n
+  | Sbind  : (pre_n : nat) -> (itm_n : nat) -> (post_n : nat) ->
+             (f : shape_tree pre_n itm_n) -> (g : shape_tree itm_n post_n) ->
+             shape_tree pre_n post_n
+  | SbindP : (pre_n : nat) -> (post_n : nat) ->
+             (g : shape_tree pre_n post_n) ->
+             shape_tree pre_n post_n
+
+let rec tree_cond_has_shape (#a : Type) (#pre : pre_t) (#post0 : post_t a) (#t : prog_tree a)
+                            (c : tree_cond t pre post0)
+                            (#post_n : nat) (s : shape_tree (L.length pre) post_n)
+  : Pure prop (requires True) (ensures fun p -> p ==> (forall (x : a) . L.length (post0 x) = post_n)) (decreases c)
+  = match c with
+  | TCspec #a #pre #post pre1 post1 frame p0 p1 ->
+                                  (match s with
+                                    | Sspec pre_n post_n frame_n p0' p1' ->
+                                      pre_n = L.length pre /\
+                                      frame_n = L.length frame /\
+                                      U.cast #(Perm.perm_f L.(length pre1)) (Perm.perm_f (pre_n + frame_n))
+                                         p0 == p0' /\
+                                     (forall (x : a) .
+                                       L.length (post  x) = post_n /\
+                                       L.length (post1 x) = post_n + frame_n /\ (* already implied ? *)
+                                       U.cast #(Perm.perm_f L.(length (post x @ frame)))
+                                               (Perm.perm_f (post_n + frame_n))
+                                         (p1 x) == p1')
+                                    | _ -> False)
+  | TCret #a pre post p           -> (match s with
+                                    | Sret n p' ->
+                                      p == p' /\
+                                     (forall (x : a) . L.length (post x) = n)
+                                    | _ -> False)
+  | TCbind #a #b pre itm post f g -> (match s with
+                                    | Sbind _ itm_n post_n s_f s_g ->
+                                      tree_cond_has_shape f s_f /\
+                                     (forall (x : a) . tree_cond_has_shape (g x) s_g) /\
+                                     (forall (y : b) . L.length (post y) = post_n)
+                                    | _ -> False)
+  | TCbindP #a #b pre post g      -> (match s with
+                                    | SbindP _ post_n s_g ->
+                                      (forall (x : a) . tree_cond_has_shape (g x) s_g) /\
+                                      (forall (y : b) . L.length (post y) = post_n)
+                                    | _ -> False)
+
+
+(**** requires / ensures *)
+
+(** return *)
+
+unfold
+let return_req (pre : pre_t) : req_t pre
+  = fun _ -> True
+
+unfold
+let return_ens (#a : Type) (x : a) (p : post_t a) : ens_t (p x) a p
+  = fun sl0 r sl1 ->
+      r == x /\ sl1 == sl0
+
+(** bind *)
+
+unfold
+let bind_req (#a : Type)
+      (#pre : pre_t) (#itm : post_t a)
+      (req_f : req_t pre) (ens_f : ens_t pre a itm)
+      (req_g : (x:a) -> req_t (itm x))
+  : req_t pre
+  = fun sl0 -> req_f sl0 /\
+      (forall (x : a) (sl1 : sl_t (itm x)) .
+        ens_f sl0 x sl1 ==> req_g x sl1)
+
+/// Unlike the bind combiner of Steel, our ensures clause does not recall the pre-condition of [f] for
+/// the reason explained on [Experiment.Repr.Fun.tree_ens]
+
+unfold
+let bind_ens (#a : Type) (#b : Type)
+      (#pre : pre_t) (#itm : post_t a) (#post : post_t b)
+      (ens_f : ens_t pre a itm) (ens_g : (x:a) -> ens_t (itm x) b post)
+  : ens_t pre b post
+  = fun sl0 y sl2 ->
+      (exists (x : a) (sl1 : sl_t (itm x)) .
+        ens_f sl0 x sl1 /\
+        ens_g x sl1 y sl2)
+
+(** bind_pure *)
+
+unfold
+let bind_pure_req (#a : Type) (wp : pure_wp a)
+      (#pre : pre_t)
+      (req : a -> req_t pre)
+  : req_t pre
+  = fun sl0 -> wp (fun x -> req x sl0) /\ True
+
+unfold
+let bind_pure_ens (#a : Type) (#b : Type)
+      (wp : pure_wp a)
+      (#pre : pre_t) (#post : post_t b)
+      (ens : a -> ens_t pre b post)
+  : ens_t pre b post
+  = fun sl0 y sl1 -> (exists (x:a) . as_ensures wp x /\ ens x sl0 y sl1)
+
+
+(** prog_tree *)
+
+let rec tree_req (#a : Type u#a) (t : prog_tree a)
+                 (#pre : pre_t) (#post : post_t a) (c : tree_cond t pre post)
+  : Tot (req_t pre) (decreases t) =
+  match c with
+  | TCspec #_ #pre #_ #req #_  pre' _ frame  p0 _ ->
+             (fun sl0 -> req (extract_vars_f pre' pre frame p0 sl0)._1)
+  | TCret #_ #_  pre _  _ ->
+             return_req pre
+  | TCbind #_ #_ #f #g  pre itm _  cf cg ->
+             bind_req (tree_req f cf) (tree_ens f cf) (fun x -> tree_req (g x) (cg x))
+  | TCbindP #_ #_ #wp #_ #g  pre _  cg ->
+             bind_pure_req wp (fun x -> tree_req (g x) (cg x))
+
+and tree_ens (#a : Type u#a) (t : prog_tree a)
+             (#pre : pre_t) (#post : post_t a) (c : tree_cond t pre post)
+  : Tot (ens_t pre a post) (decreases t) =
+  match c with
+  | TCspec #a #pre #post #req #ens  pre' post' frame  p0 p1 ->
+             (fun sl0' x sl1' ->
+                let sl0, frame0 = extract_vars_f pre' pre frame p0 sl0' in
+                let sl1, frame1 = extract_vars_f (post' x) (post x) frame
+                                                 (Perm.pequiv_sym (p1 x)) sl1' in
+                frame1 == frame0 /\ ens sl0 x sl1)
+  | TCret #a #x  pre post  p ->
+             (fun sl0 x' sl1 ->
+                x' == x /\
+               (let sl0' = extract_vars p sl0 in
+                sl1 == sl0'))
+  | TCbind #_ #_ #f #g  pre itm post  cf cg ->
+             bind_ens (tree_ens f cf) (fun x -> tree_ens (g x) (cg x))
+  | TCbindP #_ #_ #wp #_ #g  pre post  cg ->
+             bind_pure_ens wp (fun x -> tree_ens (g x) (cg x))
+
+
+(*** "Monad" *)
+
+/// We define a "monad" (which does not satisfy the monad laws) on a [repr] type which contains a representation
+/// of the program as a tree and a corresponding steel function.
+
+noeq
+type repr (a : Type) = {
+  repr_tree  : prog_tree a;
+  repr_steel : (pre : pre_t) -> (post : post_t a) -> (c : tree_cond repr_tree pre post) ->
+               repr_steel_t a pre post (tree_req repr_tree c) (tree_ens repr_tree c)
+}
+
+let tree_of_steel (#a : Type) (#pre : pre_t) (#post : post_t a) (#req : req_t pre) (#ens : ens_t pre a post)
+                  ($f : repr_steel_t a pre post req ens)
+  : prog_tree a
+  = Tspec a pre post req ens
+
+val repr_of_steel_steel
+      (a : Type) (pre : pre_t) (post : post_t a) (req : req_t pre) (ens : ens_t pre a post)
+      (pre' : pre_t) (post' : post_t a) (frame : vprop_list)
+      (p0 : vequiv pre' L.(pre @ frame)) (p1 : ((x : a) -> vequiv (post x @ frame) (post' x)))
+      ($f : repr_steel_t a pre post req ens)
+  : (let c = TCspec #a #pre #post #req #ens pre' post' frame p0 p1 in
+     repr_steel_t a pre' post' (tree_req _ c) (tree_ens _ c))
+
+[@@ __tree_reduce__]
+let repr_of_steel (#a : Type) (pre : pre_t) (post : post_t a) (req : req_t pre) (ens : ens_t pre a post)
+                  ($f : repr_steel_t a pre post req ens)
+  : repr a
+  = {
+    repr_tree  = tree_of_steel f;
+    repr_steel = (fun pre'0 post'0 c ->
+                    let (TCspec pre' post' frame  p0 p1) = c in
+                    U.cast (repr_steel_t a pre'0 post'0 (tree_req _ c) (tree_ens _ c))
+                           (repr_of_steel_steel a pre post req ens pre' post' frame p0 p1 f))
+  }
+
+
+val return_steel
+      (a : Type) (x : a)
+      (pre : pre_t) (post : post_t a)
+      (p : vequiv pre (post x))
+  : (let c = TCret #a #x pre post p in
+     repr_steel_t a pre post (tree_req _ c) (tree_ens _ c))
+
+[@@ __tree_reduce__]
+let return (#a : Type) (x :a)
+  : repr a
+  = {
+    repr_tree  = Tret a x;
+    repr_steel = (fun pre0 post0 c ->
+        let TCret pre post p = c in
+        U.cast (repr_steel_t a pre0 post0 (tree_req _ c) (tree_ens _ c))
+               (return_steel a x pre post p))
+  }
+
+
+val bind_steel
+      (a : Type) (b : Type) (f : prog_tree a) (g : (a -> prog_tree b))
+      (pre : pre_t) (itm : post_t a) (post : post_t b)
+      (cf : tree_cond f pre itm) (cg : ((x : a) -> tree_cond (g x) (itm x) post))
+      ($rf : repr_steel_t a pre itm (tree_req f cf) (tree_ens f cf))
+      ($rg : (x : a) -> repr_steel_t b (itm x) post (tree_req (g x) (cg x)) (tree_ens (g x) (cg x)))
+  : (let c = TCbind #a #b #f #g pre itm post cf cg in
+     repr_steel_t b pre post (tree_req _ c) (tree_ens _ c))
+
+[@@ __tree_reduce__]
+let bind (#a #b : Type)
+      (f : repr a) (g : a -> repr b)
+  : repr b
+  = {
+    repr_tree  = Tbind a b f.repr_tree (fun x -> (g x).repr_tree);
+    repr_steel = (fun pre0 post0 c ->
+                    let (TCbind #a' #b' #tf #tg pre itm post cf cg) = c in
+                    let rg (x : a) : repr_steel_t b (itm x) post _ _
+                                   = (g x).repr_steel _ _ (cg x) in
+                    U.cast (repr_steel_t b pre0 post0 (tree_req _ c) (tree_ens _ c))
+                           (bind_steel a b tf tg pre itm post cf cg (f.repr_steel _ _ cf) rg))
+  }
